Proving stuff for soundness

References.v
@@ -10,90 +10,90 @@ From Elo Require Import Meta.
 From Elo Require Import ValidAddresses.
 
 (* ------------------------------------------------------------------------- *)
-(* well-typed-references                                                     *)
+(* consistently-typed-references                                             *)
 (* ------------------------------------------------------------------------- *)
 
-Inductive well_typed_references (m : mem) : tm -> Prop :=
-  | wtr_unit :
-    well_typed_references m <{ unit }> 
+Inductive consistently_typed_references (m : mem) : tm -> Prop :=
+  | ctr_unit :
+    consistently_typed_references m <{ unit }> 
 
-  | wtr_num : forall n,
-    well_typed_references m <{ N n }>
+  | ctr_num : forall n,
+    consistently_typed_references m <{ N n }>
 
-  | wtr_refM : forall T ad,
+  | ctr_refM : forall T ad,
     empty |-- m[ad].tm is T ->
     m[ad].typ = <{{ &T }}> ->
-    well_typed_references m <{ &ad :: &T }>
+    consistently_typed_references m <{ &ad :: &T }>
 
-  | wtr_refI : forall T ad,
+  | ctr_refI : forall T ad,
     empty |-- m[ad].tm is <{{ Immut T }}> ->
     m[ad].typ = <{{ i&T }}> ->
-    well_typed_references m <{ &ad :: i&T }>
+    consistently_typed_references m <{ &ad :: i&T }>
 
-  | wtr_new : forall T t,
-    well_typed_references m t ->
-    well_typed_references m <{ new T t }> 
+  | ctr_new : forall T t,
+    consistently_typed_references m t ->
+    consistently_typed_references m <{ new T t }> 
 
-  | wtr_load : forall t,
-    well_typed_references m t ->
-    well_typed_references m <{ *t }> 
+  | ctr_load : forall t,
+    consistently_typed_references m t ->
+    consistently_typed_references m <{ *t }> 
 
-  | wtr_asg : forall t1 t2,
-    well_typed_references m t1 ->
-    well_typed_references m t2 ->
-    well_typed_references m <{ t1 = t2 }> 
+  | ctr_asg : forall t1 t2,
+    consistently_typed_references m t1 ->
+    consistently_typed_references m t2 ->
+    consistently_typed_references m <{ t1 = t2 }> 
 
-  | wtr_var : forall x,
-    well_typed_references m <{ var x }>
+  | ctr_var : forall x,
+    consistently_typed_references m <{ var x }>
 
-  | wtr_fun : forall x Tx t,
-    well_typed_references m t ->
-    well_typed_references m <{ fn x Tx t }>
+  | ctr_fun : forall x Tx t,
+    consistently_typed_references m t ->
+    consistently_typed_references m <{ fn x Tx t }>
 
-  | wtr_call : forall t1 t2,
-    well_typed_references m t1 ->
-    well_typed_references m t2 ->
-    well_typed_references m <{ call t1 t2 }> 
+  | ctr_call : forall t1 t2,
+    consistently_typed_references m t1 ->
+    consistently_typed_references m t2 ->
+    consistently_typed_references m <{ call t1 t2 }> 
 
-  | wtr_seq : forall t1 t2,
-    well_typed_references m t1 ->
-    well_typed_references m t2 ->
-    well_typed_references m <{ t1; t2 }>
+  | ctr_seq : forall t1 t2,
+    consistently_typed_references m t1 ->
+    consistently_typed_references m t2 ->
+    consistently_typed_references m <{ t1; t2 }>
 
-  | wtr_spawn : forall t,
-    well_typed_references m t ->
-    well_typed_references m <{ spawn t }>
+  | ctr_spawn : forall t,
+    consistently_typed_references m t ->
+    consistently_typed_references m <{ spawn t }>
   .
 
-Ltac inversion_wtr :=
-  match goal with
-  | H : well_typed_references _ <{ unit     }> |- _ => inversion H; subst
-  | H : well_typed_references _ <{ N _      }> |- _ => inversion H; subst
-  | H : well_typed_references _ <{ & _ :: _ }> |- _ => inversion H; subst
-  | H : well_typed_references _ <{ new _ _  }> |- _ => inversion H; subst
-  | H : well_typed_references _ <{ * _      }> |- _ => inversion H; subst
-  | H : well_typed_references _ <{ _ = _    }> |- _ => inversion H; subst
-  | H : well_typed_references _ <{ var _    }> |- _ => inversion H; subst
-  | H : well_typed_references _ <{ fn _ _ _ }> |- _ => inversion H; subst
-  | H : well_typed_references _ <{ call _ _ }> |- _ => inversion H; subst
-  | H : well_typed_references _ <{ _ ; _    }> |- _ => inversion H; subst
-  | H : well_typed_references _ <{ spawn _  }> |- _ => inversion H; subst
-  end.
+Ltac inversion_ctr :=
+ match goal with
+ | H : consistently_typed_references _ <{ unit     }> |- _ => inv_subst H
+ | H : consistently_typed_references _ <{ N _      }> |- _ => inv_subst H
+ | H : consistently_typed_references _ <{ & _ :: _ }> |- _ => inv_subst H
+ | H : consistently_typed_references _ <{ new _ _  }> |- _ => inv_subst H
+ | H : consistently_typed_references _ <{ * _      }> |- _ => inv_subst H
+ | H : consistently_typed_references _ <{ _ = _    }> |- _ => inv_subst H
+ | H : consistently_typed_references _ <{ var _    }> |- _ => inv_subst H
+ | H : consistently_typed_references _ <{ fn _ _ _ }> |- _ => inv_subst H
+ | H : consistently_typed_references _ <{ call _ _ }> |- _ => inv_subst H
+ | H : consistently_typed_references _ <{ _ ; _    }> |- _ => inv_subst H
+ | H : consistently_typed_references _ <{ spawn _  }> |- _ => inv_subst H
+ end.
 
-Ltac inversion_clear_wtr :=
-  match goal with
-  | H : well_typed_references _ <{ unit     }> |- _ => inversion_subst_clear H
-  | H : well_typed_references _ <{ N _      }> |- _ => inversion_subst_clear H
-  | H : well_typed_references _ <{ & _ :: _ }> |- _ => inversion_subst_clear H
-  | H : well_typed_references _ <{ new _ _  }> |- _ => inversion_subst_clear H
-  | H : well_typed_references _ <{ * _      }> |- _ => inversion_subst_clear H
-  | H : well_typed_references _ <{ _ = _    }> |- _ => inversion_subst_clear H
-  | H : well_typed_references _ <{ var _    }> |- _ => inversion_subst_clear H
-  | H : well_typed_references _ <{ fn _ _ _ }> |- _ => inversion_subst_clear H
-  | H : well_typed_references _ <{ call _ _ }> |- _ => inversion_subst_clear H
-  | H : well_typed_references _ <{ _ ; _    }> |- _ => inversion_subst_clear H
-  | H : well_typed_references _ <{ spawn _  }> |- _ => inversion_subst_clear H
-  end.
+Ltac inversion_clear_ctr :=
+ match goal with
+ | H : consistently_typed_references _ <{ unit     }> |- _ => inv_subst_clear H
+ | H : consistently_typed_references _ <{ N _      }> |- _ => inv_subst_clear H
+ | H : consistently_typed_references _ <{ & _ :: _ }> |- _ => inv_subst_clear H
+ | H : consistently_typed_references _ <{ new _ _  }> |- _ => inv_subst_clear H
+ | H : consistently_typed_references _ <{ * _      }> |- _ => inv_subst_clear H
+ | H : consistently_typed_references _ <{ _ = _    }> |- _ => inv_subst_clear H
+ | H : consistently_typed_references _ <{ var _    }> |- _ => inv_subst_clear H
+ | H : consistently_typed_references _ <{ fn _ _ _ }> |- _ => inv_subst_clear H
+ | H : consistently_typed_references _ <{ call _ _ }> |- _ => inv_subst_clear H
+ | H : consistently_typed_references _ <{ _ ; _    }> |- _ => inv_subst_clear H
+ | H : consistently_typed_references _ <{ spawn _  }> |- _ => inv_subst_clear H
+ end.
 
 (* ------------------------------------------------------------------------- *)
 (* preservation                                                              *)
@@ -103,153 +103,158 @@ Ltac inversion_clear_wtr :=
 Local Lemma step_write_wtt : forall m t t' ad v Tr T,
   empty |-- t is T ->
   t --[EF_Write ad v Tr]--> t' ->
-  well_typed_references m t ->
+  consistently_typed_references m t ->
   (Tr = m[ad].typ /\ exists V, empty |-- v is V /\ empty |-- m[ad].tm is V).
 Proof.
   intros * ? ?.
   assert (exists V, empty |-- v is V) as [? ?].
   { generalize dependent T. induction_step; intros; inversion_type; eauto. }
   intros. generalize dependent T.
-  induction_step; intros; inversion_type; inversion_wtr; eauto.
-  inversion_type. inversion_wtr. apply_deterministic_typing. eauto.
+  induction_step; intros; inversion_type; inversion_ctr; eauto.
+  inversion_type. inversion_ctr. apply_deterministic_typing. eauto.
 Qed.
 
 (* ------------------------------------------------------------------------- *)
 
-Local Lemma wtr_subst_preservation : forall m t tx x,
-  well_typed_references m t ->
-  well_typed_references m tx ->
-  well_typed_references m ([x := tx] t).
+Local Lemma ctr_subst_preservation : forall m t tx x,
+  consistently_typed_references m t ->
+  consistently_typed_references m tx ->
+  consistently_typed_references m ([x := tx] t).
 Proof.
-  intros. induction t; inversion_wtr; eauto using well_typed_references;
-  simpl; destruct string_eq_dec; subst; eauto using well_typed_references.
+  intros. induction t; inversion_ctr;
+  eauto using consistently_typed_references;
+  simpl; destruct string_eq_dec; subst;
+  eauto using consistently_typed_references.
 Qed.
 
-Local Lemma wtr_mem_add_preservation : forall m t vT,
+Local Lemma ctr_mem_add_preservation : forall m t vT,
   valid_addresses m t ->
-  well_typed_references m t ->
-  well_typed_references (m +++ vT) t.
+  consistently_typed_references m t ->
+  consistently_typed_references (m +++ vT) t.
 Proof.
-  intros * ? Hwtr. induction Hwtr;
-  try inversion_vad; eauto using well_typed_references;
-  (eapply wtr_refM || eapply wtr_refI); simpl_array; assumption.
+  intros * ? Hctr. induction Hctr;
+  try inversion_vad; eauto using consistently_typed_references;
+  (eapply ctr_refM || eapply ctr_refI); simpl_array; assumption.
 Qed.
 
-Local Lemma wtr_mem_set_preservation : forall m t ad v T,
+Local Lemma ctr_mem_set_preservation : forall m t ad v T,
   ad < #m ->
   empty |-- v is T ->
   empty |-- m[ad].tm is T ->
-  well_typed_references m t ->
-  well_typed_references m[ad <- (v, m[ad].typ)] t.
+  consistently_typed_references m t ->
+  consistently_typed_references m[ad <- (v, m[ad].typ)] t.
 Proof.
-  intros * ? ? ? Hwtr. rename ad into ad'. 
-  induction Hwtr; eauto using well_typed_references;
-  (eapply wtr_refM || eapply wtr_refI);
+  intros * ? ? ? Hctr. rename ad into ad'. 
+  induction Hctr; eauto using consistently_typed_references;
+  (eapply ctr_refM || eapply ctr_refI);
   decompose sum (lt_eq_lt_dec ad' ad); subst;
   simpl_array; trivial; apply_deterministic_typing; trivial.
 Qed.
 
 (* ------------------------------------------------------------------------- *)
 
-Local Lemma wtr_tstep_none_preservation : forall m t t',
-  well_typed_references m t ->
+Local Lemma ctr_tstep_none_preservation : forall m t t',
+  consistently_typed_references m t ->
   t --[EF_None]--> t' ->
-  well_typed_references m t'.
+  consistently_typed_references m t'.
 Proof.
-  intros. induction_step; inversion_wtr; eauto using well_typed_references.
-  inversion_wtr. eauto using wtr_subst_preservation.
+  intros. induction_step; inversion_ctr;
+  eauto using consistently_typed_references.
+  inversion_ctr. eauto using ctr_subst_preservation.
 Qed.
 
-Local Lemma wtr_tstep_alloc_preservation : forall m t t' v T,
+Local Lemma ctr_tstep_alloc_preservation : forall m t t' v T,
   well_typed_term t ->
   valid_addresses m t ->
-  well_typed_references m t ->
+  consistently_typed_references m t ->
   t --[EF_Alloc (#m) v T]--> t' ->
-  well_typed_references (m +++ (v, T)) t'.
+  consistently_typed_references (m +++ (v, T)) t'.
 Proof.
   intros * [T' ?]. intros. generalize dependent T'.
-  induction_step; intros; inversion_vad; inversion_type; inversion_wtr;
-  eauto using well_typed_references, wtr_mem_add_preservation;
-  (eapply wtr_refM || eapply wtr_refI); simpl_array; trivial.
+  induction_step; intros; inversion_vad; inversion_type; inversion_ctr;
+  eauto using consistently_typed_references, ctr_mem_add_preservation;
+  (eapply ctr_refM || eapply ctr_refI); simpl_array; trivial.
 Qed.
 
-Local Lemma wtr_tstep_read_preservation : forall m t t' ad v,
-  well_typed_references m v ->
-  well_typed_references m t ->
+Local Lemma ctr_tstep_read_preservation : forall m t t' ad v,
+  consistently_typed_references m v ->
+  consistently_typed_references m t ->
   t --[EF_Read ad v]--> t' ->
-  well_typed_references m t'.
+  consistently_typed_references m t'.
 Proof.
-  intros. induction_step; inversion_wtr; eauto using well_typed_references.
+  intros. induction_step; inversion_ctr;
+  eauto using consistently_typed_references.
 Qed.
 
-Local Lemma wtr_tstep_write_preservation : forall m t t' ad v T,
+Local Lemma ctr_tstep_write_preservation : forall m t t' ad v T,
   well_typed_term t ->
   valid_addresses m t ->
-  well_typed_references m t ->
+  consistently_typed_references m t ->
   t --[EF_Write ad v T]--> t' ->
-  well_typed_references m[ad <- (v, T)] t'.
+  consistently_typed_references m[ad <- (v, T)] t'.
 Proof.
   intros * [T' ?]. intros. assert (
     T = m[ad].typ /\
     exists Tv, empty |-- v is Tv /\ empty |-- m[ad].tm is Tv)
     as [? [? [? ?]]] by eauto using step_write_wtt.
   generalize dependent T'.
-  induction_step; intros; inversion_type; inversion_vad; inversion_wtr;
+  induction_step; intros; inversion_type; inversion_vad; inversion_ctr;
   eauto using valid_address_write,
-    well_typed_references,
-    wtr_mem_set_preservation.
+    consistently_typed_references,
+    ctr_mem_set_preservation.
 Qed.
 
-Lemma wtr_tstep_spawn_preservation : forall m t t' block,
-  well_typed_references m t ->
+Lemma ctr_tstep_spawn_preservation : forall m t t' block,
+  consistently_typed_references m t ->
   t --[EF_Spawn block]--> t' ->
-  well_typed_references m t'.
+  consistently_typed_references m t'.
 Proof.
-  intros. induction_step; inversion_wtr; eauto using well_typed_references.
+  intros. induction_step; inversion_ctr;
+  eauto using consistently_typed_references.
 Qed.
 
-Local Corollary wtr_mstep_preservation : forall m m' t t' e,
+Local Corollary ctr_mstep_preservation : forall m m' t t' e,
   well_typed_term t ->
   valid_addresses m t ->
-  forall_memory m (well_typed_references m) ->
-  well_typed_references m t ->
+  forall_memory m (consistently_typed_references m) ->
+  consistently_typed_references m t ->
   m / t ==[e]==> m' / t' ->
-  well_typed_references m' t'.
+  consistently_typed_references m' t'.
 Proof.
-  intros * ? ?. eapply mstep_preservation; (* optimization *)
-  eauto using wtr_tstep_none_preservation,
-    wtr_tstep_alloc_preservation,
-    wtr_tstep_read_preservation,
-    wtr_tstep_write_preservation.
+  solve_mstep_preservation_using
+    ctr_tstep_none_preservation
+    ctr_tstep_alloc_preservation
+    ctr_tstep_read_preservation
+    ctr_tstep_write_preservation.
 Qed.
 
 (* ------------------------------------------------------------------------- *)
 
-Local Lemma wtr_thread_default_preservation : forall m,
-  well_typed_references m thread_default.
+Local Lemma ctr_thread_default_preservation : forall m,
+  consistently_typed_references m thread_default.
 Proof.
-  eauto using well_typed_references.
+  eauto using consistently_typed_references.
 Qed.
 
-Lemma wtr_spawn_block_preservation : forall m t t' block,
-  well_typed_references m t ->
+Lemma ctr_spawn_block_preservation : forall m t t' block,
+  consistently_typed_references m t ->
   t --[EF_Spawn block]--> t' ->
-  well_typed_references m block.
+  consistently_typed_references m block.
 Proof.
-  intros. induction_step; inversion_wtr; eauto.
+  intros. induction_step; inversion_ctr; eauto.
 Qed.
 
-Local Lemma wtr_untouched_threads_preservation : forall m m' ths tid tid' e t',
+Local Lemma ctr_untouched_threads_preservation : forall m m' ths tid tid' e t',
   forall_threads ths well_typed_term ->
   forall_threads ths (valid_addresses m) ->
-  forall_threads ths (well_typed_references m) ->
+  forall_threads ths (consistently_typed_references m) ->
   tid <> tid' ->
   tid' < #ths ->
   m / ths[tid] ==[e]==> m' / t' ->
-  well_typed_references m' ths[tid'].
+  consistently_typed_references m' ths[tid'].
 Proof.
   intros *. intros Htype. intros. destruct (Htype tid).
-  inversion_mstep; eauto using wtr_mem_add_preservation.
+  inversion_mstep; eauto using ctr_mem_add_preservation.
   match goal with
   | _ : _ --[EF_Write _ _ ?T]--> _ |- _ =>
     assert (
@@ -257,24 +262,24 @@ Proof.
       exists V, empty |-- v is V /\ empty |-- m[ad].tm is V)
       as [Heq [? [? ?]]] by eauto using step_write_wtt
   end.
-  rewrite Heq in *. eauto using wtr_mem_set_preservation.
+  rewrite Heq in *. eauto using ctr_mem_set_preservation.
 Qed.
 
-Local Corollary wtr_cstep_preservation : forall m m' ths ths' tid e,
+Local Corollary ctr_cstep_preservation : forall m m' ths ths' tid e,
   forall_threads ths well_typed_term ->
   forall_threads ths (valid_addresses m) ->
-  forall_memory m (well_typed_references m) ->
-  forall_threads ths (well_typed_references m) ->
+  forall_memory m (consistently_typed_references m) ->
+  forall_threads ths (consistently_typed_references m) ->
   m / ths ~~[tid, e]~~> m' / ths' ->
-  forall_threads ths' (well_typed_references m').
+  forall_threads ths' (consistently_typed_references m').
 Proof.
   intros * Htype ?. destruct (Htype tid).
   eauto 6 using cstep_preservation,
-    wtr_tstep_spawn_preservation,
-    wtr_mstep_preservation,
-    wtr_thread_default_preservation,
-    wtr_spawn_block_preservation,
-    wtr_untouched_threads_preservation.
+    ctr_tstep_spawn_preservation,
+    ctr_mstep_preservation,
+    ctr_thread_default_preservation,
+    ctr_spawn_block_preservation,
+    ctr_untouched_threads_preservation.
 Qed.
 
 (* ------------------------------------------------------------------------- *)
@@ -288,48 +293,48 @@ Proof.
   induction_step; intros; inversion_type; eauto.
 Qed.
 
-Local Lemma wtr_alloc_value_generalization : forall m t t' ad v T,
-  well_typed_references m t ->
+Local Lemma ctr_alloc_value_generalization : forall m t t' ad v T,
+  consistently_typed_references m t ->
   t --[EF_Alloc ad v T]--> t' ->
-  well_typed_references m v.
+  consistently_typed_references m v.
 Proof.
-  intros. induction_step; intros; inversion_wtr; eauto.
+  intros. induction_step; intros; inversion_ctr; eauto.
 Qed.
 
-Local Lemma wtr_write_value_generalization : forall m t t' ad v T,
-  well_typed_references m t ->
+Local Lemma ctr_write_value_generalization : forall m t t' ad v T,
+  consistently_typed_references m t ->
   t --[EF_Write ad v T]--> t' ->
-  well_typed_references m v.
+  consistently_typed_references m v.
 Proof.
-  intros. induction_step; intros; inversion_wtr; eauto.
+  intros. induction_step; intros; inversion_ctr; eauto.
 Qed.
 
-Local Lemma wtr_tstep_alloc_mem_preservation : forall m t t' v T,
+Local Lemma ctr_tstep_alloc_mem_preservation : forall m t t' v T,
   well_typed_term t ->
   valid_addresses m t ->
   forall_memory m (valid_addresses m) ->
   (* --- *)
-  well_typed_references m t ->
-  forall_memory m (well_typed_references m) ->
+  consistently_typed_references m t ->
+  forall_memory m (consistently_typed_references m) ->
   t --[EF_Alloc (#m) v T]--> t' ->
-  forall_memory (m +++ (v, T)) (well_typed_references (m +++ (v, T))).
+  forall_memory (m +++ (v, T)) (consistently_typed_references (m +++ (v, T))).
 Proof.
   intros. intros ad.
   assert (well_typed_term v) as [? ?]
     by eauto using wtt_alloc_value_generalization.
   decompose sum (lt_eq_lt_dec ad (#m)); subst; simpl_array;
-  eauto using well_typed_references; (* optimization *)
-  eauto using wtr_mem_add_preservation, wtr_alloc_value_generalization.
+  eauto using consistently_typed_references; (* optimization *)
+  eauto using ctr_mem_add_preservation, ctr_alloc_value_generalization.
 Qed.
 
-Local Lemma wtr_tstep_write_mem_preservation : forall m t t' ad v T,
+Local Lemma ctr_tstep_write_mem_preservation : forall m t t' ad v T,
   ad < # m ->
   well_typed_term t ->
   (* --- *)
-  well_typed_references m t ->
-  forall_memory m (well_typed_references m) ->
+  consistently_typed_references m t ->
+  forall_memory m (consistently_typed_references m) ->
   t --[EF_Write ad v T]--> t' ->
-  forall_memory m[ad <- (v, T)] (well_typed_references m[ad <- (v, T)]).
+  forall_memory m[ad <- (v, T)] (consistently_typed_references m[ad <- (v, T)]).
 Proof.
   intros * ? [? ?]. intros. intros ad'.
   match goal with
@@ -340,52 +345,48 @@ Proof.
       as [? [? [? ?]]] by eauto using step_write_wtt
   end.
   decompose sum (lt_eq_lt_dec ad' ad); subst; simpl_array;
-  eauto using wtr_write_value_generalization, wtr_mem_set_preservation.
+  eauto using ctr_write_value_generalization, ctr_mem_set_preservation.
 Qed.
 
-Local Corollary wtr_mstep_mem_preservation : forall m m' t t' e,
+Local Corollary ctr_mstep_mem_preservation : forall m m' t t' e,
   well_typed_term t ->
   valid_addresses m t ->
   forall_memory m (valid_addresses m) ->
   (* --- *)
-  well_typed_references m t ->
-  forall_memory m (well_typed_references m) ->
+  consistently_typed_references m t ->
+  forall_memory m (consistently_typed_references m) ->
   m / t ==[e]==> m' / t' ->
-  forall_memory m' (well_typed_references m').
+  forall_memory m' (consistently_typed_references m').
 Proof.
-  intros. inversion_mstep;
-  eauto using wtr_tstep_alloc_mem_preservation,
-              wtr_tstep_write_mem_preservation.
+  solve_mstep_mem_preservation_using 
+    ctr_tstep_alloc_mem_preservation 
+    ctr_tstep_write_mem_preservation.
 Qed.
 
-Local Corollary wtr_cstep_mem_preservation : forall m m' ths ths' tid e,
+Local Corollary ctr_cstep_mem_preservation : forall m m' ths ths' tid e,
   forall_threads ths well_typed_term ->
   forall_threads ths (valid_addresses m) ->
   forall_memory m (valid_addresses m) ->
   (* --- *)
-  forall_threads ths (well_typed_references m) ->
-  forall_memory m (well_typed_references m) ->
+  forall_threads ths (consistently_typed_references m) ->
+  forall_memory m (consistently_typed_references m) ->
   m / ths ~~[tid, e]~~> m' / ths' ->
-  forall_memory m' (well_typed_references m').
+  forall_memory m' (consistently_typed_references m').
 Proof.
-  intros. inversion_cstep; eauto using wtr_mstep_mem_preservation.
+  solve_cstep_mem_preservation_using ctr_mstep_mem_preservation.
 Qed.
 
 (* ------------------------------------------------------------------------- *)
 
-(* TODO: consistently_typed_references *)
-
-Theorem well_typed_references_preservation : forall m m' ths ths' tid e,
+Theorem consistently_typed_references_preservation : forall m m' ths ths' tid e,
   forall_program m ths well_typed_term ->
   forall_program m ths (valid_addresses m) ->
   (* --- *)
-  forall_program m ths (well_typed_references m) ->
+  forall_program m ths (consistently_typed_references m) ->
   m / ths ~~[tid, e]~~> m' / ths' ->
-  forall_program m' ths' (well_typed_references m').
+  forall_program m' ths' (consistently_typed_references m').
 Proof.
-  intros * [_ ?] [? ?].
-  eauto using preservation,
-    wtr_cstep_preservation,
-    wtr_cstep_mem_preservation.
+  intros * [_ ?] [? ?] [? ?]. intros.
+  eauto using ctr_cstep_preservation, ctr_cstep_mem_preservation.
 Qed.
 
